progs/verif_cond_queue.v
@@ -212,34 +212,99 @@ Proof.
   rewrite Z.add_simpl_r, remove_complete; auto.
 Qed.
 
-Lemma inv_precise : forall buf len (Hbuf : isptr buf) (Hlen : isptr len),
-  precise (Interp (lock_pred buf len)).
+Lemma all_ptrs : forall reqs,
+  fold_right sepcon emp (map Interp (map (fun r => Exp _ (fun data =>
+    Data_at _ Tsh trequest (Vint (Int.repr data)) r)) reqs)) |--
+  !!(Forall isptr reqs).
 Proof.
-  simpl.
-(*  intros; apply derives_precise with (Q := data_at_ Tsh (tarray (tptr trequest) 10) buf *
-    data_at_ Tsh (tarray tint 1) len * fold_right sepcon emp (map (data_at_ Tsh trequest) ).
-       (map Interp
-          (map (fun r : val => Exp Z (fun data : Z => Data_at CompSpecs Tsh trequest (Vint (Int.repr data)) r)) x))))).
-  - intros ? (? & a1 & a2 & ? & Ha1 & ? & b & Hjoinb & Ha2 & Hemp).
-    assert (predicates_hered.app_pred emp b) as Hb.
-    { destruct Hemp as (? & ? & Hjoinb' & ((? & ?) & Hemp) & ?); simpl in *.
-      specialize (Hemp _ _ Hjoinb'); subst; auto. }
-    apply sepalg.join_comm in Hjoinb.
-    specialize (Hb _ _ Hjoinb); subst.
-    exists a1, a2; split; [auto|].
-    split; [apply (data_at_data_at_ _ _ _ _ _ Ha1) | apply (data_at_data_at_ _ _ _ _ _ Ha2)].
-  - destruct buf, len; try contradiction.
-    apply precise_sepcon; [|(*apply data_at_precise; auto*)admit].
-    intros; unfold data_at_, field_at_, field_at, at_offset; simpl.
-    apply precise_andp2.
-    rewrite data_at_rec_eq; unfold withspacer, at_offset; simpl.
-    unfold array_pred, aggregate_pred.array_pred; simpl.
-    unfold Zlength, Znth; simpl.
-    apply precise_andp2.
-    rewrite data_at_rec_eq; simpl.
-    repeat (apply precise_sepcon; [apply mapsto_undef_precise; auto|]).
-    apply precise_emp.*)
-Admitted.
+  induction reqs; simpl; intros; entailer.
+  rewrite data_at_isptr.
+  eapply derives_trans; [apply saturate_aux20|].
+  { apply andp_left1, derives_refl. }
+  { apply IHreqs; auto. }
+  normalize.
+Qed.
+
+Lemma precise_reqs : forall reqs, precise (fold_right sepcon emp (map Interp (map (fun r => Exp _ (fun d =>
+  Data_at _ Tsh trequest (Vint (Int.repr d)) r)) reqs))).
+Proof.
+  induction reqs; simpl.
+  - apply precise_emp.
+  - apply precise_sepcon; auto.
+    unfold data_at, field_at, at_offset; simpl.
+    intros ??? (? & ? & Hp1) (? & ? & Hp2) ??.
+    rewrite data_at_rec_eq in Hp1, Hp2; simpl in Hp1, Hp2.
+    unfold withspacer, at_offset in Hp1, Hp2; simpl in Hp1, Hp2.
+    rewrite by_value_data_at_rec_nonvolatile in Hp1, Hp2; auto.
+    unfold mapsto in *; simpl in *.
+    destruct a; try contradiction; simpl in *.
+    unfold unfold_reptype in *; simpl in *.
+    destruct (readable_share_dec Tsh); [|contradiction n; auto].
+    destruct Hp1 as [(? & Hp1) | (? & ?)]; [|discriminate].
+    destruct Hp2 as [(? & Hp2) | (? & ?)]; [|discriminate].
+    eapply ex_address_mapsto_precise; eauto; eexists; eauto.
+Qed.
+
+Lemma inv_precise : forall buf len, precise (Interp (lock_pred buf len)).
+Proof.
+  intros ????? (reqs1 & ? & ? & ? & Hbuf1 & ? & ? & ? & Hlen1 & ? & ? & ? & ((? & ?) & Hemp1) & Hdata1)
+    (reqs2 & ? & ? & ? & Hbuf2 & ? & ? & ? & Hlen2 & ? & ? & ? & ((? & ?) & Hemp2) & Hdata2) ??.
+  exploit (data_at_int_array_inj Ews).
+  { auto. }
+  { apply Hlen1. }
+  { apply Hlen2. }
+  { eapply sepalg.join_sub_trans; [eexists; eauto|].
+    eapply sepalg.join_sub_trans; [eexists; eauto | eauto]. }
+  { eapply sepalg.join_sub_trans; [eexists; eauto|].
+    eapply sepalg.join_sub_trans; [eexists; eauto | eauto]. }
+  { repeat constructor; auto; discriminate. }
+  { repeat constructor; auto; discriminate. }
+  intros (? & Heq); subst.
+  assert (Zlength reqs1 = Zlength reqs2) as Hlen.
+  { rewrite <- (Int.signed_repr (Zlength reqs1)), <- (Int.signed_repr (Zlength reqs2)).
+    congruence.
+    { rewrite Zlength_correct; pose proof Int.min_signed_neg; split; [omega|].
+      transitivity (Z.of_nat MAX); [Omega0 | simpl; computable]. }
+    { rewrite Zlength_correct; pose proof Int.min_signed_neg; split; [omega|].
+      transitivity (Z.of_nat MAX); [Omega0 | simpl; computable]. } }
+  pose proof (all_ptrs _ _ Hdata1) as Hptrs1.
+  pose proof (all_ptrs _ _ Hdata2) as Hptrs2.
+  exploit (data_at_ptr_array_inj Ews).
+  { auto. }
+  { apply Hbuf1. }
+  { apply Hbuf2. }
+  { eapply sepalg.join_sub_trans; [eexists; eauto | eauto]. }
+  { eapply sepalg.join_sub_trans; [eexists; eauto | eauto]. }
+  { apply Forall_complete; [|discriminate].
+    eapply Forall_impl; [|apply Hptrs1].
+    destruct a; auto; discriminate. }
+  { apply Forall_complete; [|discriminate].
+    eapply Forall_impl; [|apply Hptrs2].
+    destruct a; auto; discriminate. }
+  intros (? & Hbufs); subst.
+  assert (reqs1 = reqs2); [|subst].
+  { repeat rewrite Zlength_correct in Hlen.
+    eapply complete_inj; [eauto | omega]. }
+  exploit (precise_reqs reqs2).
+  { apply Hdata1. }
+  { apply Hdata2. }
+  { eapply sepalg.join_sub_trans; [eexists; eauto|].
+    eapply sepalg.join_sub_trans; [eexists; eauto|].
+    eapply sepalg.join_sub_trans; [eexists; eauto | eauto]. }
+  { eapply sepalg.join_sub_trans; [eexists; eauto|].
+    eapply sepalg.join_sub_trans; [eexists; eauto|].
+    eapply sepalg.join_sub_trans; [eexists; eauto | eauto]. }
+  intro; subst.
+  match goal with H1 : predicates_hered.app_pred emp ?a,
+    H2 : predicates_hered.app_pred emp ?b |- _ => assert (a = b);
+      [eapply sepalg.same_identity; auto;
+        [match goal with H : sepalg.join a ?x ?y |- _ =>
+           specialize (Hemp1 _ _ H); subst; eauto end |
+         match goal with H : sepalg.join b ?x ?y |- _ =>
+           specialize (Hemp2 _ _ H); subst; eauto end] | subst] end.
+  repeat match goal with H1 : sepalg.join ?a ?b ?c, H2 : sepalg.join ?a ?b ?d |- _ =>
+    pose proof (sepalg.join_eq H1 H2); clear H1 H2; subst end; auto.
+Qed.
 
 Lemma inv_positive : forall buf len,
   positive_mpred (Interp (lock_pred buf len)).
@@ -259,7 +324,7 @@ Proof.
   forward_call tt.
   Intro x; destruct x as (r, data).
   forward_call (lock, sh, lock_pred buf len).
-  { destruct lock; try contradiction; simpl; entailer. }
+  { destruct lock; try contradiction; simpl; entailer'. }
   simpl.
   Intro reqs; normalize.
   forward.
@@ -276,11 +341,12 @@ Proof.
         lock_inv sh lock (Interp (lock_pred buf len));
         @data_at CompSpecs Tsh trequest (Vint (Int.repr data)) r;
         cond_var sh cprod; cond_var sh ccon)).
-  (* Unfortunately, Delta now contains an equality involving unfold_reptype that causes a discriminate
+  (* XX Delta now contains an equality involving unfold_reptype that causes a discriminate
      in fancy_intros (in saturate_local) to go into an infinite loop. *)
   - Exists reqs; go_lower; entailer'.
   - go_lower; entailer'.
   - forward_call (cprod, lock, sh, sh, lock_pred buf len).
+    { destruct lock; try contradiction; simpl; entailer'. }
     { simpl.
       Exists reqs0; unfold fold_right at 3; cancel.
       entailer'; cancel. }
@@ -298,8 +364,9 @@ Proof.
     rewrite data_at_isptr, field_at_isptr; normalize.
     rewrite (data_at_isptr _ trequest); normalize.
     forward_call (lock, sh, lock_pred buf len).
+    { destruct lock; try contradiction; simpl; entailer'. }
     { simpl.
-      Exists (reqs0 ++ [r]); timeout 10 cancel.
+      Exists (reqs0 ++ [r]); cancel.
       unfold fold_right at 2; unfold fold_right at 1; cancel.
       unfold upd_Znth; simpl.
       rewrite sublist.sublist_nil.
@@ -328,6 +395,7 @@ Proof.
     [|forward; entailer].
   forward.
   forward_call (lock, sh, lock_pred buf len).
+  { destruct lock; try contradiction; simpl; entailer. }
   simpl.
   Intro reqs; normalize.
   forward.
@@ -345,6 +413,7 @@ Proof.
   - Exists reqs; entailer.
   - entailer.
   - forward_call (ccon, lock, sh, sh, lock_pred buf len).
+    { destruct lock; try contradiction; simpl; entailer. }
     { simpl.
       Exists reqs0; entailer!.
       unfold fold_right at 1; cancel. }
@@ -366,6 +435,7 @@ Proof.
     forward.
     rewrite data_at_isptr, field_at_isptr; normalize.
     forward_call (lock, sh, lock_pred buf len).
+    { destruct lock; try contradiction; simpl; entailer. }
     { simpl.
       Exists (removelast reqs0); entailer!.
       unfold upd_Znth; simpl.
@@ -382,6 +452,15 @@ Proof.
     forward_call (last reqs0 (Vint (Int.repr 0)), data).
     { simpl; cancel. }
     unfold fold_right; entailer!.
+Qed.
+
+Lemma lock_struct : forall p, data_at_ Ews (Tstruct _lock_t noattr) p |-- data_at_ Ews tlock p.
+Proof.
+  intros.
+  unfold data_at_, field_at_, field_at; simpl; entailer.
+  unfold default_val; simpl.
+  rewrite data_at_rec_eq; simpl.
+  unfold struct_pred, aggregate_pred.struct_pred, at_offset, withspacer; simpl; entailer.
 Qed.
 
 Lemma body_main:  semax_body Vprog Gprog f_main main_spec.
@@ -423,7 +502,8 @@ Proof.
              (repeat (Vint (Int.repr 0)) (Z.to_nat i) ++ repeat Vundef (Z.to_nat (10 - i))) gvar4;
          data_at_ Ews tint gvar3; data_at_ Ews tint gvar2;
          data_at_ Ews (tarray tint 1) gvar1; data_at_ Ews tlock gvar0)).
-  { unfold tlock, semax_conc._lock_t, trequest, _request_t; entailer!. }
+  { unfold trequest, _request_t; entailer!.
+    apply sepcon_derives; [entailer | apply lock_struct]. }
   { forward.
     entailer!.
     assert (Zlength (repeat (Vint (Int.repr 0)) (Z.to_nat i)) = i) as Hlen.
@@ -443,8 +523,10 @@ Proof.
     rewrite Hminus; simpl; omega. }
   forward.
   forward_call (gvar0, Ews, lock_pred gvar4 gvar1).
+  { destruct gvar0; try contradiction; simpl; entailer. }
   rewrite (data_at_isptr _ (tarray _ _)), field_at_isptr; normalize.
   forward_call (gvar0, Ews, lock_pred gvar4 gvar1).
+  { destruct gvar0; try contradiction; simpl; entailer. }
   { simpl.
     Exists ([] : list val); simpl; entailer!. }
   { split; auto; split.
@@ -509,12 +591,14 @@ Proof.
   { entailer. }
   { (* loop body *)
     forward_call (gvar3, gvar0, sh2, sh2, lock_pred gvar4 gvar1).
+    { destruct gvar0; try contradiction; simpl; entailer. }
     { simpl; cancel.
       Exists reqs0; unfold fold_right at 1; cancel; entailer!. }
     simpl; Intro reqs'; normalize.
     forward.
     Exists reqs'; entailer!. }
   forward_call (gvar0, sh2, lock_pred gvar4 gvar1).
+  { destruct gvar0; try contradiction; simpl; entailer. }
   { simpl; Exists reqs0; cancel.
     unfold fold_right at 1; entailer!. }
   { split; auto; split; [apply inv_precise | apply inv_positive]; auto. }
