progs/verif_incr.v
@@ -68,20 +68,13 @@ Definition main_spec :=
 Definition Gprog : funspecs := augment_funspecs prog [acquire_spec; release_spec; release2_spec; makelock_spec;
   freelock_spec; freelock2_spec; spawn_spec; incr_spec; read_spec; thread_func_spec; main_spec].
 
-Lemma ctr_inv_precise : forall b o,
-  predicates_sl.precise (EX x : Z, data_at Ews (tarray tint 1) [Vint (Int.repr x)] (Vptr b o)).
+Lemma ctr_inv_precise : forall p,
+  predicates_sl.precise (EX x : Z, data_at Ews (tarray tint 1) [Vint (Int.repr x)] p).
 Proof.
-  intros; apply predicates_sl.derives_precise with (Q := data_at_ Ews (tarray tint 1) (Vptr b o)).
-  { intros ? (? & ?).
-    apply (data_at_data_at_ _ _ _ _ _ H). }
-  unfold data_at_, field_at_, field_at, at_offset; simpl.
-  apply precise_andp2.
-  rewrite data_at_rec_eq; unfold withspacer, at_offset; simpl.
-  unfold array_pred, aggregate_pred.array_pred; simpl.
-  unfold Zlength, Znth; simpl.
-  apply precise_andp2.
-  rewrite data_at_rec_eq; simpl.
-  apply precise_sepcon; [apply mapsto_undef_precise | apply precise_emp]; auto.
+  intros ???? (? & ?) (? & ?) ??.
+  eapply data_at_int_array_inj; try eassumption; auto.
+  { repeat constructor; auto; discriminate. }
+  { repeat constructor; auto; discriminate. }
 Qed.
 
 Lemma ctr_inv_positive : forall ctr,
@@ -151,6 +144,15 @@ Qed.
 
 Definition thread_lock_pred' sh ctr lockc lockt := Later (Self_lock (Lock_inv sh lockc (lock_pred ctr)) sh lockt).
 
+Lemma lock_struct : forall p, data_at_ Ews (Tstruct _lock_t noattr) p |-- data_at_ Ews tlock p.
+Proof.
+  intros.
+  unfold data_at_, field_at_, field_at; simpl; entailer.
+  unfold default_val; simpl.
+  rewrite data_at_rec_eq; simpl.
+  unfold struct_pred, aggregate_pred.struct_pred, at_offset, withspacer; simpl; entailer.
+Qed.
+
 Lemma body_main:  semax_body Vprog Gprog f_main main_spec.
 Proof.
   start_function.
@@ -179,20 +181,19 @@ Proof.
   forward.
   forward_call (gvar0, Ews, lock_pred gvar2).
   { destruct gvar0; try contradiction; simpl; entailer. }
-  { subst Frame; instantiate (1 := [field_at Ews (tarray tint 1) [] [Vint (Int.repr 0)] gvar2;
-      data_at_ Ews (Tstruct 2%positive noattr) gvar1]); admit. }
+  { rewrite (sepcon_comm _ (fold_right _ _ _)); apply sepcon_derives; [cancel | apply lock_struct]. }
   rewrite field_at_isptr; normalize.
   forward_call (gvar0, Ews, lock_pred gvar2).
   { destruct gvar0; try contradiction; simpl; entailer. }
-  { subst Frame; instantiate (1 := [data_at_ Ews tlock gvar1]); simpl.
-    unfold tlock, semax_conc._lock_t; entailer!.
-    Exists 0; entailer!. admit. }
+  { simpl.
+    Exists 0; cancel. }
   { destruct gvar2; try contradiction.
     split; auto; split; [apply ctr_inv_precise | apply ctr_inv_positive]. }
   (* need to split off shares for the locks here *)
   destruct split_Ews as (sh1 & sh2 & ? & ? & Hsh).
   forward_call (gvar1, Ews, thread_lock_pred sh1 gvar2 gvar0 gvar1).
   { destruct gvar1; try contradiction; simpl; entailer. }
+  { rewrite (sepcon_comm _ (fold_right _ _ _)); apply sepcon_derives; [cancel | apply lock_struct]. }
   get_global_function'' _thread_func.
   normalize.
   apply extract_exists_pre; intros f_.
@@ -255,7 +256,7 @@ Proof.
   { unfold cptr_lock_inv; simpl; entailer!. }
   { split; [auto | apply ctr_inv_positive]. }
   forward.
-Admitted.
+Qed.
 
 Definition extlink := ext_link_prog prog.
 
